tests/wp.v
@@ -1,3 +1,0 @@
-From complete_iris.program_logic Require Import weakestpre.
-
-Print Assumptions hoare_requisiteness_nofork.
